sepcomp/closed_safety.v
@@ -1,0 +1,106 @@
+Require Import sepcomp.compcert. Import CompcertLibraries.
+
+Require Import sepcomp.core_semantics.
+
+Set Implicit Arguments.
+Unset Strict Implicit.
+Unset Printing Implicit Defensive.
+
+Section closed_safety.
+
+Variable (G C D Z M : Type).
+
+Variable sem : CoreSemantics G C M.
+
+Variable ge : G.
+
+Fixpoint safeN (n : nat) (c : C) (m : M) : Prop :=
+  match n with
+    | O => True
+    | S n' => 
+      match halted sem c with
+        | None => 
+          exists c', exists m',
+            corestep sem ge c m c' m' /\
+            safeN n' c' m'
+        | Some i => True
+      end
+  end.
+
+Lemma safe_downward1 n c m : safeN (S n) c m -> safeN n c m.
+Proof.
+revert c m; induction n; simpl; intros; auto.
+destruct (halted sem c); auto.
+destruct H as [c' [m' [? ?]]].
+exists c', m'; split; auto.
+Qed.
+
+Lemma safe_downward (n n' : nat) c m :
+  le n' n -> safeN n c m -> safeN n' c m.
+Proof.
+do 2 intro. revert c m H0. induction H; auto.
+intros. apply IHle. apply safe_downward1. auto.
+Qed.
+
+Lemma safe_corestep_forward c m c' m' n :
+  corestep_fun sem -> 
+  corestep sem ge c m c' m' -> safeN (S n) c m -> 
+  safeN n c' m'.
+Proof.
+simpl; intros.
+erewrite corestep_not_halted in H1; eauto.
+destruct H1 as [c'' [m'' [? ?]]].
+assert ((c',m') = (c'',m'')).
+destruct (H _ _ _ _ _ _ _ H0 H1).
+subst; auto.
+inv H3; auto.
+Qed.
+
+Lemma safe_corestepN_forward c m c' m' n n0 :
+  corestep_fun sem -> 
+  corestepN sem ge n0 c m c' m' -> 
+  safeN (n + S n0) c m -> safeN n c' m'.
+Proof.
+intros.
+revert c m c' m' n H0 H1.
+induction n0; intros; auto.
+simpl in H0; inv H0.
+eapply safe_downward in H1; eauto. omega.
+simpl in H0. destruct H0 as [c2 [m2 [STEP STEPN]]].
+apply (IHn0 _ _ _ _ n STEPN). 
+assert (Heq: (n + S (S n0) = S (n + S n0))%nat) by omega.
+rewrite Heq in H1.
+eapply safe_corestep_forward in H1; eauto.
+Qed.
+
+Lemma safe_corestep_backward c m c' m' n :
+  corestep sem ge c m c' m' -> 
+  safeN (n - 1) c' m' -> 
+  safeN n c m.
+Proof.
+simpl; intros.
+induction n; simpl; auto.
+erewrite corestep_not_halted; eauto.
+exists c', m'; split; auto.
+assert (Heq: (n = S n - 1)%nat) by omega.
+rewrite Heq; auto.
+Qed.
+
+Lemma safe_corestepN_backward c m c' m' n n0 :
+  corestepN sem ge n0 c m c' m' -> 
+  safeN (n - n0) c' m' -> 
+  safeN n c m.
+Proof.
+simpl; intros.
+revert c m c' m' n H H0.
+induction n0; intros; auto.
+simpl in H; inv H.
+solve[assert (Heq: (n = n - 0)%nat) by omega; rewrite Heq; auto].
+simpl in H. destruct H as [c2 [m2 [STEP STEPN]]].
+assert (H: safeN (n - 1 - n0) c' m'). 
+eapply safe_downward in H0; eauto. omega.
+specialize (IHn0 _ _ _ _ (n - 1)%nat STEPN H). 
+eapply safe_corestep_backward; eauto.
+Qed.
+
+End closed_safety.
