sepcomp/compcert.v
@@ -1,0 +1,18 @@
+Module CompcertLibraries.
+Require Export compcert.lib.Coqlib.
+Require Export compcert.lib.Maps.
+Require Export compcert.lib.Integers.
+End CompcertLibraries.
+
+Module CompcertCommon.
+Require Export compcert.common.Events.
+Require Export compcert.common.Memory.
+Require Export compcert.common.Values.
+Require Export compcert.common.AST.
+Require Export compcert.common.Globalenvs.
+End CompcertCommon.
+
+Module CompcertAll.
+Export CompcertLibraries.
+Export CompcertCommon.
+End CompcertAll.
